First version of induction in the symbolic eval

src/Symbolic/Symbolic.v
@@ -1,5 +1,5 @@
 From CoreErlang.FrameStack Require Import SubstSemantics SubstSemanticsLemmas.
-From CoreErlang.Interpreter Require Import StepFunctions.
+From CoreErlang.Interpreter Require Import StepFunctions Equivalences.
 
 Open Scope string_scope.
 Import ListNotations.
@@ -40,12 +40,22 @@ Ltac case_innermost :=
   | |- ?g => case_innermost_term g
   end.
 
+Ltac case_innermost_in H :=
+  let T := type of H in
+  case_innermost_term T.
+
+Tactic Notation "case_innermost" :=
+  case_innermost.
+
+Tactic Notation "case_innermost" ident(H) :=
+  case_innermost_in H.
+
 Fixpoint ssmkInner (fs : FrameStack) (r : Redex) (n : nat) : FrameStack * Redex :=
   match sequentialStepFunc fs r with
   | None => (fs, r)
   | Some (fs', r') =>
     match n with
-    | 0 => (fs', r')
+    | 0 => (fs, r)
     | S n' => ssmkInner fs' r' n'
     end
   end.
@@ -56,7 +66,7 @@ Definition isEnd (fs : FrameStack) (r : Redex) : bool :=
   | _, _ => false
   end.
 
-Fixpoint ssmk2 (fs : FrameStack) (r : Redex) (n : nat) : FrameStack * Redex :=
+Fixpoint ssmk (fs : FrameStack) (r : Redex) (n : nat) : FrameStack * Redex :=
 match isEnd fs r with
 | true => (fs, r)
 | false =>
@@ -64,17 +74,17 @@ match isEnd fs r with
   | 0 => (fs, r)
   | S n' => 
     let (fs', r') := ssmkInner fs r 1000 in
-    ssmk2 fs' r' n'
+    ssmk fs' r' n'
   end
 end.
 
 Arguments ssmkInner !_ !_ !_ /.
-Arguments ssmk2 !_ !_ !_ /.
+Arguments ssmk !_ !_ !_ /.
 
 Ltac simpl_and_try_solve :=
   simpl;                                          (* simplify the goal *)
   lazymatch goal with
-  | [ |- context[ssmk2] ] => try lia              (* eval not done: is the case impossible? *)
+  | [ |- context[ssmk] ] => try lia              (* eval not done: is the case impossible? *)
   | _ => try (eexists; split;[reflexivity|nia])   (* eval done: the result exists & postcond holds *)
   end.
 
@@ -84,49 +94,9 @@ Ltac solve_forward :=
 
 
 Theorem fact_eval_example:
-  forall (z : Z), (0 <= z < 30)%Z -> exists (y : Z), ssmk2 [] (fact_frameStack (˝VLit z)) 1000 = ([], RValSeq [VLit y]) /\ (z <= y)%Z.
+  forall (z : Z), (0 <= z < 10)%Z -> exists (y : Z), ssmk [] (fact_frameStack (˝VLit z)) 1000 = ([], RValSeq [VLit y]) /\ (z <= y)%Z.
 Proof.
   intros. unfold fact_frameStack.
-  all:simpl_and_try_solve.
-  case_innermost.
-  all:simpl_and_try_solve.
-  case_innermost.
-  all:simpl_and_try_solve.
-  case_innermost.
-  all:simpl_and_try_solve.
-  case_innermost.
-  all:simpl_and_try_solve.
-  case_innermost.
-  all:simpl_and_try_solve.
-  case_innermost.
-  all:simpl_and_try_solve.
-  case_innermost.
-  all:simpl_and_try_solve.
-  case_innermost.
-  all:simpl_and_try_solve.
-  case_innermost.
-  all:simpl_and_try_solve.
-  case_innermost.
-  all:simpl_and_try_solve.
-  case_innermost.
-  all:simpl_and_try_solve.
-  case_innermost.
-  all:simpl_and_try_solve.
-  case_innermost.
-  all:simpl_and_try_solve.
-  case_innermost.
-  all:simpl_and_try_solve.
-  case_innermost.
-  all:simpl_and_try_solve.
-  case_innermost.
-  all:simpl_and_try_solve.
-  case_innermost.
-  all:simpl_and_try_solve.
-  case_innermost.
-  all:simpl_and_try_solve.
-  case_innermost.
-  all:simpl_and_try_solve.
-  case_innermost.
   all:simpl_and_try_solve.
   case_innermost.
   all:simpl_and_try_solve.
@@ -151,12 +121,630 @@ Proof.
 Qed.
 
 Theorem fact_eval_example':
-  forall (z : Z), (0 <= z < 30)%Z -> exists (y : Z), ssmk2 [] (fact_frameStack (˝VLit z)) 1000 = ([], RValSeq [VLit y]) /\ (z <= y)%Z.
+  forall (z : Z), (0 <= z < 30)%Z -> exists (y : Z), ssmk [] (fact_frameStack (˝VLit z)) 1000 = ([], RValSeq [VLit y]) /\ (z <= y)%Z.
 Proof.
   intros; unfold fact_frameStack.
   solve_forward.
 Qed.
 
+Theorem fact_eval_example_rec0:
+  forall (z : Z), (0 <= z)%Z -> 
+  exists (y : Z), ssmk [] (fact_frameStack (˝VLit z)) 1000 = ([], RValSeq [VLit y]) /\ (z <= y)%Z.
+Proof.
+Abort.
+
+Lemma ssmkInnerTrans:
+  forall (fs fs' fs'' : FrameStack) (r r' r'' : Redex) (n n' : nat),
+  ssmkInner fs r n = (fs', r') -> ssmkInner fs' r' n' = (fs'', r'') -> ssmkInner fs r (n + n') = (fs'', r'').
+Proof.
+  intros fs fs' fs'' r r' r'' n. revert fs fs' fs'' r r' r''.
+  induction n; intros.
+  * simpl. unfold ssmkInner in H. destruct (sequentialStepFunc fs r); try destruct p; inv H; auto.
+  * simpl. unfold ssmkInner. unfold ssmkInner in H.
+    destruct (sequentialStepFunc fs r) eqn:Hssf.
+    + destruct p. fold ssmkInner in *. eapply IHn; eauto.
+    + inv H.
+      destruct n'.
+      - unfold ssmkInner in H0. rewrite Hssf in H0. auto.
+      - unfold ssmkInner in H0. rewrite Hssf in H0. auto.
+Qed.
+
+Lemma ssmkInnerLet:
+  forall (fs: FrameStack) (r: Redex) (n n' : nat),
+  ssmkInner fs r (n + n') = let (fs', r') := ssmkInner fs r n in ssmkInner fs' r' n'.
+Proof.
+  intros. revert fs r n'. induction n; intros.
+  * simpl. destruct (ssmkInner fs r 0) eqn:HssmkInner.
+    unfold ssmkInner in HssmkInner.
+    destruct (sequentialStepFunc fs r) eqn:Hssf.
+    1:destruct p. all:inv HssmkInner. all:auto.
+  * simpl.
+    unfold ssmkInner. destruct (sequentialStepFunc fs r) eqn:Hssf.
+    1:destruct p. all:fold ssmkInner.
+    + auto.
+    + destruct n'.
+      all:unfold ssmkInner.
+      all:rewrite Hssf.
+      all:auto.
+Qed.
+
+Theorem ssmkEquiv:
+  forall (fs : FrameStack) (r : Redex) (n : nat),
+  ssmk fs r n = ssmkInner fs r (n * 1000).
+Proof.
+  intros fs r n. revert fs r.
+  induction n; intros.
+  + simpl. unfold ssmk, ssmkInner.
+    destruct (isEnd fs r).
+    all:destruct (sequentialStepFunc fs r).
+    1,3:destruct p. all:reflexivity.
+  + rewrite Nat.mul_succ_l.
+    unfold ssmk. destruct (isEnd fs r) eqn:HisEnd.
+    - unfold isEnd in *. destruct fs; try discriminate. destruct r; try discriminate.
+      rewrite Nat.add_comm. simpl. reflexivity.
+    - fold ssmk.
+      destruct (ssmkInner fs r 1000) eqn:Hssmk.
+      rewrite Nat.add_comm.
+      rewrite ssmkInnerLet. rewrite Hssmk. auto.
+Qed.
+
+Lemma ssmkTrans:
+  forall (fs fs' fs'' : FrameStack) (r r' r'' : Redex) (n n' : nat),
+  ssmk fs r n = (fs', r') -> ssmk fs' r' n' = (fs'', r'') -> ssmk fs r (n + n') = (fs'', r'').
+Proof.
+  setoid_rewrite ssmkEquiv.
+  intros.
+  assert ((n + n') * 1000 = (n * 1000 + n' * 1000)) by lia.
+  rewrite H1. clear H1.
+  eapply ssmkInnerTrans; eauto.
+Qed.
+
+Lemma backOneInner:
+  forall (fs fs' fs'' : FrameStack) (r r' r'' : Redex) (n n' : nat),
+  ssmkInner fs r 1 = (fs', r') ->
+  (let (fs0, r0) := ssmkInner fs' r' n in ssmk fs0 r0 n' = (fs'', r'')) ->
+  let (fs0, r0) := ssmkInner fs r (S n) in ssmk fs0 r0 n' = (fs'', r'').
+Proof.
+  intros.
+  destruct (ssmkInner fs' r' n) eqn:HssmkInner.
+  rewrite ssmkEquiv in H0.
+  destruct (ssmkInner fs r (S n)) eqn:HssmkInner0.
+  rewrite ssmkEquiv.
+  assert (S n = 1 + n) by lia.
+  rewrite H1 in HssmkInner0. clear H1.
+  rewrite ssmkInnerLet in HssmkInner0.
+  rewrite H in HssmkInner0.
+  rewrite HssmkInner0 in HssmkInner. inv HssmkInner. auto.
+Qed.
+
+Lemma advanceOneInner:
+  forall (fs fs'' : FrameStack) (r r'' : Redex) (n n' : nat),
+  (let (fs0, r0) := ssmkInner fs r (S n) in ssmk fs0 r0 n' = (fs'', r'')) ->
+  exists (fs' : FrameStack) (r' : Redex),
+    ssmkInner fs r 1 = (fs', r') /\
+    (let (fs0, r0) := ssmkInner fs' r' n in ssmk fs0 r0 n' = (fs'', r'')).
+Proof.
+  intros.
+  destruct (ssmkInner fs r (S n)) eqn:HssmkInner.
+  rewrite ssmkEquiv in H.
+  assert (S n = 1 + n) by lia.
+  rewrite H0 in HssmkInner. clear H0.
+  rewrite ssmkInnerLet in HssmkInner.
+  destruct (ssmkInner fs r 1) eqn:HssmkInner0.
+  do 2 eexists. split. eauto.
+  rewrite HssmkInner.
+  rewrite ssmkEquiv. auto.
+Qed.
+
+Lemma backOnePivot:
+  forall (fs fs' fs'' : FrameStack) (r r' r'' : Redex) (n : nat),
+  ssmkInner fs r 1 = (fs', r') ->
+  ssmk fs' r' n = (fs'', r'') ->
+  let (fs0, r0) := ssmkInner fs r 1 in ssmk fs0 r0 n = (fs'', r'').
+Proof.
+  intros. rewrite H. auto.
+Qed.
+
+Lemma advanceOnePivot:
+  forall (fs fs'' : FrameStack) (r r'' : Redex) (n : nat),
+  (let (fs0, r0) := ssmkInner fs r 1 in ssmk fs0 r0 n = (fs'', r'')) ->
+  exists (fs' : FrameStack) (r' : Redex),
+    ssmkInner fs r 1 = (fs', r') /\
+    ssmk fs' r' n = (fs'', r'').
+Proof.
+  intros. setoid_rewrite ssmkEquiv.
+  destruct (ssmkInner fs r 1) eqn:HssmkInner.
+  rewrite ssmkEquiv in H.
+  do 2 eexists. split. eauto. auto.
+Qed.
+
+Lemma backOneChange:
+  forall (fs fs' fs'' : FrameStack) (r r' r'' : Redex) (n : nat),
+  ssmkInner fs r 1 = (fs', r') ->
+  (let (fs0, r0) := ssmkInner fs' r' 999 in ssmk fs0 r0 n = (fs'', r'')) ->
+  ssmk fs r (S n) = (fs'', r'').
+Proof.
+  intros.
+  rewrite ssmkEquiv.
+  destruct (ssmkInner fs' r' 999) eqn:HssmkInner.
+  rewrite ssmkEquiv in H0.
+  assert (S n * 1000 = 1 + (999 + n * 1000)) by lia.
+  rewrite H1. clear H1.
+  rewrite ssmkInnerLet. rewrite H.
+  rewrite ssmkInnerLet. rewrite HssmkInner. auto.
+Qed.
+
+Lemma advanceOneChange:
+  forall (fs fs'' : FrameStack) (r r'' : Redex) (n : nat),
+  ssmk fs r (S n) = (fs'', r'') ->
+  exists (fs' : FrameStack) (r' : Redex),
+    ssmkInner fs r 1 = (fs', r') /\
+    (let (fs0, r0) := ssmkInner fs' r' 999 in ssmk fs0 r0 n = (fs'', r'')).
+Proof.
+  intros. rewrite ssmkEquiv in H.
+  assert (S n * 1000 = 1 + (999 + n * 1000)) by lia.
+  rewrite H0 in H. clear H0.
+  rewrite ssmkInnerLet in H.
+  destruct (ssmkInner fs r 1) eqn:HssmkInner.
+  rewrite ssmkInnerLet in H.
+  destruct (ssmkInner f r0 999) eqn:HssmkInner0.
+  do 2 eexists. split. eauto.
+  rewrite HssmkInner0. rewrite ssmkEquiv. auto.
+Qed.
+
+Lemma ssmkInnerOneMore:
+  forall (fs : FrameStack) (r : Redex) (v : list Val) (n : nat),
+  ssmkInner fs r n = ([], RValSeq v) -> ssmkInner fs r (S n) = ([], RValSeq v).
+Proof.
+  intros fs r v n. revert fs r v.
+  induction n; intros.
+  * unfold ssmkInner in *.
+    destruct (sequentialStepFunc fs r) eqn:Hssf.
+    1:destruct p. all:inv H. reflexivity.
+  * unfold ssmkInner. unfold ssmkInner in H.
+    destruct (sequentialStepFunc fs r) eqn:Hssf. all:auto.
+    destruct p. fold ssmkInner in *.
+    apply IHn in H.
+    unfold ssmkInner in H. destruct (sequentialStepFunc f r0) eqn:Hssf0.
+    1:destruct p. 1:fold ssmkInner in H. all:auto.
+Qed.
+
+Theorem ssmkInnerMore:
+  forall (fs : FrameStack) (r : Redex) (v : list Val) (n n' : nat),
+  n <= n' ->
+  ssmkInner fs r n = ([], RValSeq v) -> ssmkInner fs r n' = ([], RValSeq v).
+Proof.
+  intros fs r v n. revert fs r v.
+  induction n; intros.
+  * destruct n'.
+    all:unfold ssmkInner in *.
+    all:destruct (sequentialStepFunc fs r) eqn:Hssf.
+    1,3:destruct p.
+    all:auto. inv H0.
+  * destruct n'.
+    + inv H.
+    + assert (n <= n') by lia.
+      unfold ssmkInner. unfold ssmkInner in H0.
+      destruct (sequentialStepFunc fs r) eqn:Hssf.
+      - destruct p. fold ssmkInner in *.
+        apply IHn. lia. auto.
+      - auto.
+Qed.
+
+Ltac advanceOne H :=
+  first [ apply advanceOneChange in H;destruct H as [fs' [r' [Hfirst H]]];inv Hfirst
+        | apply advanceOneInner in H;destruct H as [fs' [r' [Hfirst H]]];inv Hfirst
+        | apply advanceOnePivot in H;destruct H as [fs' [r' [Hfirst H]]];inv Hfirst
+        | idtac "Nothing to advance"].
+
+Theorem fact_eval_rec:
+  forall (z : nat), (* (0 <= z) -> *)
+  forall (y : nat), ssmk [] (fact_frameStack (˝VLit (Z.of_nat z))) 1000 = ([], RValSeq [VLit (Z.of_nat y)]) ->
+  (z <= y).
+Proof.
+  intros. unfold fact_frameStack in H.
+  advanceOne H.
+  advanceOne H.
+  advanceOne H.
+  advanceOne H.
+  advanceOne H.
+  advanceOne H.
+  
+  
+  induction z.
+  * simpl in H. inv H. nia.
+  * (*simpl in H0. simpl in IHz.*)
+    advanceOne H.
+    advanceOne H.
+    advanceOne H.
+    advanceOne H.
+    advanceOne H.
+    advanceOne H.
+    advanceOne H.
+    advanceOne H.
+    advanceOne H.
+    advanceOne H.
+    advanceOne H.
+    advanceOne H.
+    advanceOne H.
+    advanceOne H.
+    advanceOne H.
+    advanceOne H.
+    advanceOne H.
+    advanceOne H.
+    advanceOne H.
+    advanceOne H.
+    advanceOne H.
+    advanceOne H.
+
+    
+    assert ((Z.of_nat (S z) - 1)%Z = Z.of_nat z) by lia.
+    rewrite H0 in H. clear H0.
+    
+    
+  
+  
+
+
+Abort.
+
+Lemma help:
+  forall (fs : FrameStack) (r r' : Redex),
+  is_result r' ->
+  (exists n, ssmk fs r (S n) = ([], r')) <->
+  exists n, ssmk fs r n = ([], r').
+Proof.
+  intros. split; intro.
+  * destruct H0. exists (S x). auto.
+  * destruct H0. destruct x.
+    + unfold ssmk in *.
+      destruct (isEnd fs r) eqn:HisEnd.
+      - inv H0. exists 0. reflexivity.
+      - fold ssmk. inv H0.
+        inv H. simpl. exists 0. simpl. reflexivity.
+    + exists x. auto.
+Qed.
+
+Definition mayRec (fs : FrameStack) (r : Redex) : bool :=
+  match fs with
+  | FParams (IApp (VClos (_ :: _) _ _ _)) _ _ :: _ => 
+    match r with
+    | RValSeq _ => true
+    | _ => false
+    end
+  | _ => false
+  end.
+
+Compute mayRec [FParams
+         (IApp
+            (VClos
+               [(0, 1,
+                 ° ECase (˝ VVar 1)
+                     [([PLit 0%Z], ˝ VLit "true", ˝ VLit 1%Z);
+                      ([PVar], ˝ VLit "true",
+                       ° ELet 1
+                           (° EApp (˝ VFunId (1, 1))
+                                [° ECall (˝ VLit "erlang") (˝ VLit "-")
+                                     [˝ VVar 0; ˝ VLit 1%Z]])
+                           (° ECall (˝ VLit "erlang") (˝ VLit "*") [˝ VVar 1; ˝ VVar 0]))])]
+               0 1
+               (° ECase (˝ VVar 1)
+                    [([PLit 0%Z], ˝ VLit "true", ˝ VLit 1%Z);
+                     ([PVar], ˝ VLit "true",
+                      ° ELet 1
+                          (° EApp (˝ VFunId (1, 1))
+                               [° ECall (˝ VLit "erlang") (˝ VLit "-") [˝ VVar 0; ˝ VLit 1%Z]])
+                          (° ECall (˝ VLit "erlang") (˝ VLit "*") [˝ VVar 1; ˝ VVar 0]))])))
+         [] []] (RValSeq [VLit (Z.of_nat 1)]).
+
+Fixpoint ssmkMayRec (fs : FrameStack) (r : Redex) (n : nat) : FrameStack * Redex * nat :=
+match mayRec fs r with
+| true => (fs, r, n)
+| false => 
+  match sequentialStepFunc fs r with
+  | None => (fs, r, n)
+  | Some (fs', r') =>
+    match n with
+    | 0 => (fs, r, n)
+    | S n' => ssmkMayRec fs' r' n'
+    end
+  end
+end.
+
+Compute ssmkMayRec [] (fact_frameStack (˝VLit 4%Z)) 100.
+
+Theorem ssmkRec:
+  forall (fs : FrameStack) (r : Redex) (n : nat),
+  ssmkInner fs r n =
+  let '(fs', r', n') := ssmkMayRec fs r n in ssmkInner fs' r' n'.
+Proof.
+  intros. revert fs r. induction n; intros.
+  * simpl. unfold ssmkInner.
+    destruct (mayRec fs r).
+    + reflexivity.
+    + destruct (sequentialStepFunc fs r) eqn:Hssf.
+      - destruct p. rewrite Hssf. reflexivity.
+      - rewrite Hssf. reflexivity.
+  * simpl. unfold ssmkInner.
+    destruct (mayRec fs r).
+    + reflexivity.
+    + destruct (sequentialStepFunc fs r) eqn:Hssf.
+      - fold ssmkInner. destruct p. auto.
+      - rewrite Hssf. reflexivity.
+Qed.
+
+Theorem fact_eval_example_rec0:
+  forall (z : nat), (*(0 <= z) -> *)
+  exists (y : nat),
+  (exists (n : nat), ssmk [] (fact_frameStack (˝VLit (Z.of_nat z))) n = ([], RValSeq [VLit (Z.of_nat y)])) 
+    /\ (z <= y).
+Proof.
+  intros. setoid_rewrite <- help;[|constructor].
+  
+  Opaque ssmkInner. simpl.
+  setoid_rewrite ssmkRec. simpl.
+  Transparent ssmkInner.
+
+Abort.
+
+(* Ltac toPotentialRec :=
+  Opaque ssmkInner; simpl; try (setoid_rewrite ssmkRec); simpl; Transparent ssmkInner.
+ *)
+
+Fixpoint ssmkInnerNoSimpl (fs : FrameStack) (r : Redex) (n : nat) : FrameStack * Redex :=
+  match sequentialStepFunc fs r with
+  | None => (fs, r)
+  | Some (fs', r') =>
+    match n with
+    | 0 => (fs, r)
+    | S n' => ssmkInnerNoSimpl fs' r' n'
+    end
+  end.
+
+Arguments ssmkInnerNoSimpl : simpl never.
+
+Lemma ssmkInnerSimplEquiv : 
+  forall (fs : FrameStack) (r : Redex) (n : nat),
+  ssmkInner fs r n = ssmkInnerNoSimpl fs r n.
+Proof. reflexivity. Qed.
+
+Theorem ssmkSimpl :
+  forall (fs : FrameStack) (r : Redex) (n : nat),
+  match isEnd fs r with
+  | true => (fs, r)
+  | false => let (fs', r') := ssmkInnerNoSimpl fs r 1000 in ssmk fs' r' n
+  end = ssmk fs r (S n).
+Proof. reflexivity. Qed.
+
+Theorem ssmkRecNoSimpl :
+  forall (fs : FrameStack) (r : Redex) (n : nat),
+  ssmkInner fs r n =
+  let '(fs', r', n') := ssmkMayRec fs r n in ssmkInnerNoSimpl fs' r' n'.
+Proof.
+  intros. rewrite ssmkRec. destruct (ssmkMayRec fs r n). destruct p. rewrite ssmkInnerSimplEquiv. reflexivity.
+Qed.
+
+Ltac toPotentialRec :=
+match goal with
+| |- context[ssmkInner] => idtac
+| _ => try (setoid_rewrite <- ssmkSimpl); simpl
+end;
+  try (setoid_rewrite ssmkRecNoSimpl); simpl;
+  try (setoid_rewrite <- ssmkInnerSimplEquiv).
+
+Lemma asd:
+  forall (fs : FrameStack) (r : Redex) (n : nat),
+  ssmkInner fs r (S n) = let (fs', r') := ssmkInner fs r 1 in ssmkInnerNoSimpl fs' r' n.
+Proof. Admitted.
+
+Theorem fact_eval_example_rec0:
+  forall (z : nat), (*(0 <= z) -> *)
+  exists (y : Z),
+  (exists (n : nat), ssmk [] (fact_frameStack (˝VLit (Z.of_nat z))) n = ([], RValSeq [VLit y])) 
+    /\ ((Z.of_nat z) <= y)%Z.
+Proof.
+  intros. setoid_rewrite <- help;[|constructor].
+  toPotentialRec.
+  induction z.
+  * simpl. eexists. split;[exists 0;reflexivity|nia].
+  * setoid_rewrite asd. simpl. setoid_rewrite <- ssmkInnerSimplEquiv.
+    toPotentialRec. setoid_rewrite ssmkInnerSimplEquiv. unfold eval_arith_NEW. simpl.
+    remember (IApp _). clear Heqf.
+
+Abort.
+
+Theorem ssmkInnerOuter:
+  forall (fs : FrameStack) (r r': Redex) (k : nat),
+  is_result r' ->
+  (exists n, (let (fs0, r0) := ssmkInner fs r k in ssmk fs0 r0 n) = ([], r')) <->
+  (exists n, ssmk fs r n = ([], r')).
+Proof.
+  intros. split.
+  * intros.
+    destruct H0. destruct (ssmkInner fs r k) eqn:HssmkInner.
+    setoid_rewrite ssmkEquiv.
+    rewrite ssmkEquiv in H0.
+    exists (x + k).
+    assert ((x + k) * 1000 = k + ((x * 1000) + (k * 999))) by lia.
+    rewrite H1. clear H1.
+    rewrite ssmkInnerLet. rewrite HssmkInner.
+    rewrite ssmkInnerLet. rewrite H0.
+    inv H.
+    + destruct k; simpl; reflexivity.
+    + destruct k; simpl; reflexivity.
+  * intros.
+    destruct H0.
+    (* setoid_rewrite not working backwards?? *)
+    assert 
+    ( (exists n : nat, (let (fs0, r0) := ssmkInner fs r k in ssmkInner fs0 r0 (n * 1000)) = ([], r')) ->
+      (exists n : nat, (let (fs0, r0) := ssmkInner fs r k in ssmk fs0 r0 n) = ([], r'))).
+    { intros. destruct (ssmkInner fs r k). setoid_rewrite ssmkEquiv. auto. }
+    apply H1. clear H1.
+    (* setoid_rewrite not working backwards again??? *)
+    assert
+    ( (∃ n : nat, ssmkInner fs r (k + n * 1000) = ([], r')) ->
+      (∃ n : nat, (let (fs0, r0) := ssmkInner fs r k in ssmkInner fs0 r0 (n * 1000)) = ([], r'))).
+    { intros. setoid_rewrite ssmkInnerLet in H1. destruct (ssmkInner fs r k). auto. }
+    apply H1. clear H1.
+    rewrite ssmkEquiv in H0.
+    exists x.
+    assert (k + x * 1000 = x * 1000 + k) by lia.
+    rewrite H1. clear H1.
+    rewrite ssmkInnerLet. rewrite H0.
+    inv H.
+    + destruct k; simpl; reflexivity.
+    + destruct k; simpl; reflexivity.
+Qed.
+
+Theorem ssmkOuterIsInner:
+  forall (fs : FrameStack) (r r': Redex),
+  is_result r' ->
+  (exists n, ssmk fs r n = ([], r')) <->
+  (exists n, ssmkInner fs r n = ([], r')).
+Proof.
+  intros. split; intro.
+  * destruct H0. exists (x * 1000). rewrite <- ssmkEquiv. auto.
+  * destruct H0.
+    exists x. rewrite ssmkEquiv.
+    assert (x * 1000 = x + x * 999) by lia.
+    rewrite H1. clear H1.
+    rewrite ssmkInnerLet. rewrite H0.
+    inv H.
+    + destruct x; simpl; reflexivity.
+    + destruct x; simpl; reflexivity.
+Qed.
+
+Print frame_indep_core.
+Close Scope string_scope.
+
+Fixpoint ssExactlyk (fs : FrameStack) (r : Redex) (n : nat) : option (FrameStack * Redex) :=
+match n with
+| 0 => Some (fs, r)
+| S n' =>
+  match sequentialStepFunc fs r with
+  | Some (fs', r') => ssExactlyk fs' r' n'
+  | _ => None
+  end
+end.
+
+Theorem kStepEquiv:
+  forall (fs fs' : FrameStack) (r r' : Redex) (k : nat),
+  ⟨ fs, r ⟩ -[k]-> ⟨ fs', r' ⟩ <-> ssExactlyk fs r k = Some (fs', r').
+Proof.
+  intros. split.
+  * revert fs fs' r r'.
+    induction k; intros.
+    + simpl. inv H. reflexivity.
+    + simpl. destruct (sequentialStepFunc fs r) eqn:Hssf.
+      - destruct p. apply IHk.
+        inv H. apply sequentialStepEquiv in H1. rewrite Hssf in H1. inv H1. auto.
+      - inv H. apply sequentialStepEquiv in H1. rewrite H1 in Hssf. discriminate.
+  * revert fs fs' r r'.
+    induction k; intros.
+    + simpl in H. inv H. constructor.
+    + simpl in H. destruct (sequentialStepFunc fs r) eqn:Hssf.
+      - destruct p. apply sequentialStepEquiv in Hssf.
+        econstructor. eauto. apply IHk. auto.
+      - discriminate.
+Qed.
+
+Theorem kStepMaxkStep:
+  forall (fs fs' : FrameStack) (r r' : Redex),
+  (exists n, ssmkInner fs r n = (fs', r')) <->
+  (exists n, ssExactlyk fs r n = Some (fs', r')).
+Proof.
+  intros. split.
+  * intro. destruct H. revert H. revert fs fs' r r'.
+    induction x; intros.
+    + unfold ssmkInner in H. destruct (sequentialStepFunc fs r).
+      - destruct p. inv H. exists 0. reflexivity.
+      - inv H. exists 0. reflexivity.
+    + unfold ssmkInner in H.
+      destruct (sequentialStepFunc fs r) eqn:Hssf; fold ssmkInner in H.
+      - destruct p. apply IHx in H. destruct H. exists (S x0). simpl. rewrite Hssf. auto.
+      - inv H. exists 0. reflexivity.
+  * intro. destruct H. exists x.
+    revert H. revert fs fs' r r'.
+    induction x; intros.
+    + simpl in H. inv H. unfold ssmkInner.
+      destruct (sequentialStepFunc _ _). 1:destruct p. all:reflexivity.
+    + simpl in H. unfold ssmkInner.
+      destruct (sequentialStepFunc fs r) eqn:Hssf.
+      - destruct p. fold ssmkInner. apply IHx. auto.
+      - inv H.
+Qed.
+
+Theorem frame_indep_core_functional:
+  forall (fs fs' : FrameStack) (r r' : Redex),
+  (exists n, ssmkInner fs r n = (fs', r')) ->
+  forall (fsapp : FrameStack), (exists n, ssmkInner (fs ++ fsapp) r n = (fs' ++ fsapp, r')).
+Proof.
+  intros.
+  apply kStepMaxkStep. apply kStepMaxkStep in H.
+  destruct H. apply kStepEquiv in H.
+  exists x. apply kStepEquiv. apply frame_indep_core. auto.
+Qed.
+
+Theorem ssmkTransitive:
+  forall (fs fs' fs'' : FrameStack) (r r' r'' : Redex),
+  (exists n, ssmkInner fs r n = (fs', r')) ->
+  (exists n, ssmkInner fs' r' n = (fs'', r'')) ->
+  (exists n, ssmkInner fs r n = (fs'', r'')).
+Proof.
+  setoid_rewrite kStepMaxkStep. setoid_rewrite <- kStepEquiv. intros.
+  destruct H. destruct H0. exists (x + x0).
+  eapply transitive_eval; eauto.
+Qed.
+
+Theorem fact_eval_example_rec0':
+  forall (z : nat), (*(0 <= z) -> *)
+  exists (y : Z),
+  (exists (n : nat), ssmk [] (fact_frameStack (˝VLit (Z.of_nat z))) n = ([], RValSeq [VLit y])) 
+    /\ ((Z.of_nat z) <= y)%Z.
+Proof.
+  intros.
+  setoid_rewrite <- help;[|constructor].
+  toPotentialRec.
+  induction z.
+  * simpl. eexists. split;[exists 0;reflexivity|nia].
+  * setoid_rewrite asd. simpl. setoid_rewrite <- ssmkInnerSimplEquiv.
+    toPotentialRec. setoid_rewrite ssmkInnerSimplEquiv. unfold eval_arith_NEW. simpl.
+    remember (IApp _).
+    setoid_rewrite <- ssmkInnerSimplEquiv.
+    setoid_rewrite ssmkInnerOuter;[|constructor].
+    setoid_rewrite ssmkOuterIsInner;[|constructor].
+    setoid_rewrite ssmkInnerOuter in IHz;[|constructor].
+    setoid_rewrite ssmkOuterIsInner in IHz;[|constructor].
+    
+    destruct IHz. destruct H.
+    remember (FLet _ _) as l.
+    pose proof frame_indep_core_functional.
+    specialize (H1 _ _ _ _ H [l]). simpl in H1.
+    
+    assert ((Z.of_nat (S z) - 1)%Z = Z.of_nat z) by lia. rewrite H2. clear H2.
+    
+    eexists. split.
+    eapply ssmkTransitive. eauto.
+    subst l.
+    setoid_rewrite <- ssmkOuterIsInner;[|constructor].
+    setoid_rewrite <- help;[|constructor]. simpl.
+    exists 0. simpl. reflexivity.
+    
+    (* we actually also need the info, that 0! > 0, which is surprising... *)
+    setoid_rewrite <- ssmkOuterIsInner in H;[|constructor].
+    setoid_rewrite <- help in H;[|constructor].
+    destruct z.
+    + subst f. simpl in H. destruct H. destruct x0.
+      - simpl in H. inv H. lia.
+      - simpl in H. inv H. lia.
+    + nia.
+Qed.
+
+(* TODO
+   - look into: frame_indep_core for function
+   - look into: how do I use the old tactics for this method?
+   - look into: how can I use the new theorems for this method?
+ *)
 
 
 
